src/Subst.v
@@ -13,329 +13,168 @@ Require Import List.
 Import ListNotations.
 
 
-Inductive substitution (s : expr) (x : string) : expr -> expr -> Prop :=
-  | S_Var_Eq :
-      substitution s x (E_Var x) s
-  | S_Var_Neq :
-      ∀ (y : string), x <> y -> substitution s x (E_Var y) (E_Var y)
-  | S_App : 
-      ∀ (e1 e1' e2 e2' : expr),
-      substitution s x e1 e1' ->
-      substitution s x e2 e2' ->
-      substitution s x (E_App e1 e2) (E_App e1' e2')
-  | S_Fun_Eq : 
-      ∀ (t : type) (e : expr),
-      substitution s x (E_Fun x t e) (E_Fun x t e)
-  | S_Fun_Neq : 
-      ∀ (y: string) (t : type) (e e' : expr),
-      x <> y ->
-      closed s ->
-      substitution s x e e' -> 
-      substitution s x (E_Fun y t e) (E_Fun y t e')
-  | S_True : 
-      substitution s x E_True E_True
-  | S_False : 
-      substitution s x E_False E_False
-  | S_If : 
-      ∀ (e1 e1' e2 e2' e3 e3' : expr),
-      substitution s x e1 e1' ->
-      substitution s x e2 e2' ->
-      substitution s x e3 e3' ->
-      substitution s x (E_If e1 e2 e3) (E_If e1' e2' e3')
-  | S_Let_Eq : 
-      ∀ (e1 e1' e2 : expr),
-      substitution s x e1 e1' -> 
-      substitution s x (E_Let x e1 e2) (E_Let x e1' e2)
-  | S_Let_Neq : 
-      ∀ (y : string) (e1 e1' e2 e2': expr),
-      x <> y ->
-      closed s ->
-      substitution s x e1 e1' -> 
-      substitution s x e2 e2' -> 
-      substitution s x (E_Let y e1 e2) (E_Let y e1' e2')
+
+(* TODO: voir si on repasse à une propriété inductive pour l'hypothèse s clos qui est nécessaire *)
+Fixpoint sub  (s : expr) (x : string) (e: expr) := 
+  match e with 
+  | <{#y}> => if (x =? y)%string then s else e
+  | <{ e₁ e₂}> => <{`sub s x e₁` `sub s x e₂`}>
+  | <{fun y : t => e}> => 
+      if (x =? y)%string 
+      then <{fun y : t => e}>
+      else <{fun y : t => `sub s x e`}>
+
+  | <{true}> => <{true}>
+  | <{false}> => <{false}>
+  | <{if e₁ then e₂ else e₃}> => <{if `sub s x e₁` then `sub s x e₂` else `sub s x e₃`}>
   
-  | S_Num : 
-      ∀ (z : Z),
-      substitution s x (E_Num z) (E_Num z)
-  | S_Minus :
-      ∀ (e1 e1' e2 e2': expr),
-      substitution s x e1 e1' -> 
-      substitution s x e2 e2' -> 
-      substitution s x (E_Minus e1 e2) (E_Minus e1' e2')
+  | <{let y = e₁ in e₂}> =>
+        if (x =? y)%string 
+        then <{let y = `sub s x e₁` in e₂}>
+        else <{let y = `sub s x e₁` in `sub s x e₂`}>
 
-  | S_Eq :
-      ∀ (e1 e1' e2 e2': expr),
-      substitution s x e1 e1' -> 
-      substitution s x e2 e2' -> 
-      substitution s x (E_Eq e1 e2) (E_Eq e1' e2')
-  
-  | S_Pair : 
-      ∀ (e1 e1' e2 e2': expr),
-      substitution s x e1 e1' -> 
-      substitution s x e2 e2' -> 
-      substitution s x (E_Pair e1 e2) (E_Pair e1' e2')
-  | S_First :
-      ∀ (e e': expr),
-      substitution s x e e' -> 
-      substitution s x (E_First e) (E_First e')
-  | S_Second :
-      ∀ (e e': expr),
-      substitution s x e e' -> 
-      substitution s x (E_Second e) (E_Second e')
+  | E_Num z => E_Num z
+  | <{ e₁ - e₂}> => <{`sub s x e₁` - `sub s x e₂`}>
+  | <{ e₁ == e₂}> => <{`sub s x e₁` == `sub s x e₂`}>
 
-  | S_Record_Nil : 
-      substitution s x E_Record_Nil E_Record_Nil
-    
-  | S_Record_Cons :
-    ∀ y e e' tail tail',
-    substitution s x tail tail' ->
-    substitution s x e e' ->
-    substitution s x (E_Record_Cons y e tail) (E_Record_Cons y e' tail')
-  
-  | S_Record_Access :
-    ∀ y e e',
-    substitution s x e e' ->
-    substitution s x (E_Record_Access e y) (E_Record_Access e' y)
+  | <{ (e₁, e₂)}> => <{(`sub s x e₁`, `sub s x e₂`)}>
+  | <{first e}> => <{first `sub s x e`}>
+  | <{second e}> => <{second `sub s x e`}>
 
-  | S_Fix :
-    ∀ e e',
-    substitution s x e e' -> 
-    substitution s x (E_Fix e) (E_Fix e')
+  | <{ { lse } }> => <{ { `sub_lse s x lse` } }>
+  | <{e::v}> => <{`sub s x e` :: v}>
+  | <{fix e}> => <{fix `sub s x e`}>
 
-  | S_In_Left :
-      ∀ t₁ t₂ e e', 
-      substitution s x e e' ->
-      substitution s x (E_In_Left t₁ t₂ e) (E_In_Left t₁ t₂ e')
-  
-  | S_In_Right :
-      ∀ t₁ t₂ e e', 
-      substitution s x e e' ->
-      substitution s x (E_In_Right t₁ t₂ e) (E_In_Right t₁ t₂ e')
-
-  | S_Match :
-      ∀ e₁ e₂ e₃ e₁' e₂' e₃', 
-      substitution s x e₁ e₁' ->
-      substitution s x e₂ e₂' ->
-      substitution s x e₃ e₃' ->
-      substitution s x (E_Match e₁ e₂ e₃) (E_Match e₁' e₂' e₃')
-
-  | S_Unit : substitution s x E_Unit E_Unit
-  
-  | S_Sum_Constr :
-      ∀ constr e e',
-      substitution s x e e' ->
-      substitution s x (E_Sum_Constr constr e) (E_Sum_Constr constr e')
-
-  | S_Sum_Match :
-      ∀ e e' branches branches',
-      substitution s x e e' ->
-      substitution_lsexpr s x branches branches' -> 
-      substitution s x
-        (E_Sum_Match e branches) 
-        (E_Sum_Match e' branches')
-  
-  | S_Exc : 
-      ∀ exc, substitution s x (E_Exception exc) (E_Exception exc)
-
-with substitution_lsexpr (s : expr) (x : string) : lsexpr -> lsexpr -> Prop :=
-  | S_LSExpr_Nil : substitution_lsexpr s x LSE_Nil LSE_Nil
-  | S_LSExpr_Cons :
-    ∀ constr e e' branches branches', 
-    substitution s x e e' ->
-    substitution_lsexpr s x branches branches' ->
-    substitution_lsexpr s x 
-      (LSE_Cons constr e branches)
-      (LSE_Cons constr e' branches')
-.
-
-Hint Constructors substitution : local_hints.
-Hint Constructors substitution_lsexpr : local_hints.
-
-Check expr_ind.
-
-Fixpoint lookup_constr (constr : string) (branches : lsexpr) : option expr :=
-  match branches with
-  | LSE_Nil => None
-  | LSE_Cons constr' e tail =>
-      if (constr =? constr')%string 
-      then Some e 
-      else lookup_constr constr tail
-  end.
-
-
-Local Lemma exists_one : 
-  ∀ e s x, closed s -> 
-  ∃ e', substitution s x e e'.
-Proof with eauto with local_hints.
-  intros.
-  pose (
-    P (e : expr) :=
-      ∃ e', substitution s x e e'
-  ).
-  pose (
-    P0 (branches : lsexpr) :=
-      ∃ branches', substitution_lsexpr s x branches branches'
-  ).
-  apply expr_mut_ind with (P := P) (P0 := P0); unfold P; unfold P0; intros;
-  try (
-    try destruct H0; 
-    try destruct H1; 
-    try destruct H2;
-    try destruct (String.eqb_spec x x0); subst; 
-    eauto with local_hints; 
-    fail
-  ).
-Qed.
-
-Hint Resolve exists_one : local_hints.
-Search (_ = _ -> S _ = S _).
-
-Local Theorem deterministic :
-  ∀ e s x e'₁ e'₂, 
-  substitution s x e e'₁ ->
-  substitution s x e e'₂ ->
-  e'₁ = e'₂.
-Proof.
-  intro e.
-  pose (
-    P (e: expr) :=
-      ∀ s x e'₁ e'₂, 
-        substitution s x e e'₁ ->
-        substitution s x e e'₂ ->
-        e'₁ = e'₂
-  ).
-  pose (
-    P0 (branches: lsexpr) :=
-      ∀ s x branches'₁ branches'₂, 
-        substitution_lsexpr s x branches branches'₁ ->
-        substitution_lsexpr s x branches branches'₂ ->
-        branches'₁ = branches'₂
-  ).
-
-  apply expr_mut_ind with (P := P) (P0 := P0); unfold P; unfold P0; clear P P0;
-  try (
-    intros * H_s_1 H_s_2; inversion H_s_1; inversion H_s_2; subst;
-    eauto with local_hints;
-    try contradiction;
-    f_equal;
-    eapply IH; eauto with local_hints;
-    fail
-  );
-  try (
-    intros * IH * H_s_1 H_s_2; inversion H_s_1; inversion H_s_2; subst;
-    eauto with local_hints;
-    try contradiction;
-    f_equal;
-    eapply IH; eauto with local_hints;
-    fail
-  );
-  try (
-    intros * IH1 * IH2 * H_s_1 H_s_2; 
-    inversion H_s_1; inversion H_s_2; subst; 
-    eauto with local_hints;
-    try contradiction;
-    f_equal;
-    try (eapply IH1; eauto with local_hints; fail);
-    try (eapply IH2; eauto with local_hints; fail);
-    fail
-  );
-  try (
-    intros * IH1 * IH2 * IH3 * H_s_1 H_s_2; 
-    inversion H_s_1; inversion H_s_2; subst;
-    eauto with local_hints;
-    try contradiction; 
-    f_equal;
-    try (eapply IH1; eauto with local_hints; fail);
-    try (eapply IH2; eauto with local_hints; fail);
-    try (eapply IH3; eauto with local_hints; fail);
-    fail
-  ).
-  intros * H_s_1 H_s_2.
-  inversion H_s_1. inversion H_s_2; subst. destruct exc. destruct exc0. reflexivity.
-Qed.
-
+  | <{inl <t₁ | t₂> e}> => <{inl <t₁ | t₂> `sub s x e`}>
+  | <{inr <t₁ | t₂> e}> => <{inr <t₁ | t₂> `sub s x e`}>
+  | <{match e with | inl => eₗ | inr => eᵣ end}> => <{
+        match `sub s x e` with 
+        | inl => `sub s x eₗ` 
+        | inr => `sub s x eᵣ` 
+        end
+      }> 
+  | <{ unit }> => <{ unit }>
+  | E_Sum_Constr constr e => E_Sum_Constr constr (sub s x e)
+  | <{match_sum e with branches : default end_sum}> => <{
+        match_sum `sub s x e` with 
+        `sub_lse s x branches` 
+        : `sub s x default` 
+        end_sum
+      }> 
+  end
+  with 
+    sub_lse (s : expr) (x : string) (lse : lsexpr) : lsexpr :=
+      match lse with 
+      | <{ nil }> => <{ nil }>
+      | <{ y := e; tail }> => <{ y := `sub s x e` ; `sub_lse s x tail` }>
+      end 
+  .
+Hint Unfold sub : local_hints.
+Hint Unfold sub_lse : local_hints.
 
 Local Theorem preserves_typing : 
-  ∀ e Γ Σ s x e' t_e t_s, 
-  has_type Σ (x |-> t_s; Γ)  e  t_e -> 
-  has_type Σ empty  s  t_s -> 
-  substitution s x e e' -> 
-  has_type Σ Γ e' t_e. 
+  ∀ e Σ Γ s x tₑ tₛ, 
+  Σ / empty |- s : tₛ -> 
+  Σ / (x |-> tₛ; Γ) |- e : tₑ -> 
+  Σ / Γ |- `sub s x e` : tₑ. 
 Proof with eauto with local_hints.
   intro e.
   pose (
     P (e: expr) :=
-      ∀ Γ Σ s x e' t_e t_s, 
-      has_type Σ (x |-> t_s; Γ)  e  t_e -> 
-      has_type Σ empty  s  t_s -> 
-      substitution s x e e' -> 
-      has_type Σ Γ e' t_e
+      ∀ Σ Γ s x tₑ tₛ, 
+    Σ / empty |- s : tₛ -> 
+    Σ / (x |-> tₛ; Γ) |- e : tₑ -> 
+    Σ / Γ |- `sub s x e` : tₑ
   ).
   pose (
     P0 (branches: lsexpr) :=
-      ∀ name_sum Γ Σ s x branches' t_branches t_s, 
-      has_type_lsexpr name_sum Σ (x |-> t_s; Γ) branches t_branches -> 
-      has_type Σ empty s t_s -> 
-      substitution_lsexpr s x branches branches' -> 
-      has_type_lsexpr name_sum Σ Γ branches' t_branches
+      ∀ Σ Γ s x tₛ,
+      Σ / empty |- s : tₛ -> 
+      (
+        ∀ name_sum t,
+        Σ / (x |-> tₛ; Γ) |-ₛ name_sum ~> branches : t -> 
+        Σ / Γ |-ₛ name_sum ~> `sub_lse s x branches` : t
+      ) /\ (
+        ∀ t,
+        Σ / (x |-> tₛ; Γ) |-ᵣ branches : t -> 
+        Σ / Γ |-ᵣ `sub_lse s x branches` : t
+      )
   ).
 
   apply expr_mut_ind with (P := P) (P0 := P0); unfold P; unfold P0;
   clear P P0;
   try (
-    intros * H_type_e H_type_s H_subst;
-    inversion H_subst; inversion H_type_e; subst;
+    intros * IH1 * IH2 * IH3 * H_type_s H_type_e;
+    inversion H_type_e; subst;
     eauto with local_hints;
     fail
   );
   try (
-    intros * IH * H_type_e H_type_s H_subst;
-    inversion H_subst; inversion H_type_e; subst;
+    intros * IH1 * IH2 * H_type_s H_type_e;
+    inversion H_type_e; subst;
     eauto with local_hints;
     fail
   );
   try (
-    intros * IH1 * IH2 * H_type_e H_type_s H_subst;
-    inversion H_subst; inversion H_type_e; subst;
+    intros * IH * H_type_s H_type_e;
+    inversion H_type_e; subst;
     eauto with local_hints;
     fail
   );
   try (
-    intros * IH1 * IH2 * IH3 * H_type_e H_type_s H_subst;
-    inversion H_subst; inversion H_type_e; subst;
+    intros * H_type_s H_type_e ;
+    inversion H_type_e; subst;
     eauto with local_hints;
     fail
   ).
-  - intros * H_type_e H_type_s H_subst.
-    inversion H_subst;
-    inversion H_type_e; inversion H4; subst.
-    + rewrite String.eqb_refl in *. inversion H7; subst...
-    + apply T_Var. rewrite <- H5. symmetry; apply Maps.update_neq...
-  - intros * IH * H_type_e H_type_s H_subst.
-    inversion H_subst;
+  - intros * H_type_s H_type_e.
     inversion H_type_e; subst.
-    + apply T_Fun.
-      apply Types.weakening_eq with (Γ₁ := (x |-> t; x |-> t_s; Γ))...
+    destruct (String.eqb_spec x0 x).
+    + subst. inversion H2. simpl. rewrite String.eqb_refl in *. 
+      inversion H0; subst...
+    + simpl. rewrite <- String.eqb_neq in n. inversion H2. rewrite n in *...
+  - intros * IH1 * H_type_s H_type_e.
+    inversion H_type_e; subst.
+    simpl.
+    destruct (String.eqb_spec x0 x).
+    + apply T_Fun; subst.
+      apply Types.weakening_eq with (Γ₁ := (x |-> t; x |-> tₛ; Γ))...
       apply Maps.update_shadow.
     + apply T_Fun.
-      assert (has_type Σ (x0 |-> t_s; x |-> t; Γ) e0 t2) 
+      assert (has_type Σ (x0 |-> tₛ; x |-> t; Γ) e0 t₂) 
       by (
-        apply Types.weakening_eq with (x |-> t; x0 |-> t_s; Γ);
+        apply Types.weakening_eq with (x |-> t; x0 |-> tₛ; Γ);
         try apply Maps.update_permute; eauto with local_hints
       )...
-  - intros * IH1 * IH2 * H_type_e H_type_s H_subst.
-    inversion H_subst;
+  - intros * IH1 * IH2 * H_type_s H_type_e.
     inversion H_type_e; subst.
+    simpl.
+    destruct (String.eqb_spec x0 x).
+    + eapply T_Let; subst.
+      * eapply IH1...
+      * apply Types.weakening_eq with ((x |-> t₁; x |-> tₛ; Γ))...
+        apply Maps.update_shadow...
     + eapply T_Let.
       * eapply IH1...
-      * apply Types.weakening_eq with ((x |-> t1; x |-> t_s; Γ));
-        try apply Maps.update_shadow...
-    + eapply T_Let.
-      * eapply IH1...
-      * assert (has_type Σ (x0 |-> t_s; x |-> t1; Γ) e2 t_e)
+      * assert (has_type Σ (x0 |-> tₛ; x |-> t₁; Γ) e2 tₑ)
         by (
-          apply Types.weakening_eq with (x |-> t1; x0 |-> t_s; Γ);
+          apply Types.weakening_eq with (x |-> t₁; x0 |-> tₛ; Γ);
           try apply Maps.update_permute; eauto with local_hints
         )...  
+  - intros * IH1 * H_type_s H_type_e.
+    simpl.
+    inversion H_type_e; subst.
+    apply T_Recordt.
+    destruct (IH1 Σ Γ s x tₛ H_type_s) as [_ IH]...
+  - intros * IH1 * IH2 * IH3 * H_type_s H_type_e.
+    inversion H_type_e.
+    destruct (IH3 Σ Γ s x tₛ H_type_s) as [IH2_rec IH2_sum]...
+  - intros * H_type_s.
+    split; intros * H_type_nil...
+    inversion H_type_nil... 
+  - intros * IH1 * IH2 * H_type_s.
+    split; intros * H_type_cons; simpl;
+    inversion H_type_cons; subst;
+    destruct (IH2 Σ Γ s0 x tₛ H_type_s) as [IH2_rec IH2_sum]...
 Qed.
 Hint Resolve preserves_typing : local_hints.
