to_rewrite/okay/Step.v
@@ -11,258 +11,290 @@ Import Maps.Notations.
 
 Reserved Notation "x --> y" (at level 70, no associativity).
 Reserved Notation "x -->ₗ y" (at level 70, no associativity).
+
 Inductive step : expr -> expr -> Prop := 
   | ST_App_Fun : 
-        ∀ (x : string) (t : type) (e v : expr),
-        value v -> 
-        <{(fun x : t => e) v}> --> sub v x e
-
+      ∀ (x : string) (t : type) (e e' v : expr),
+      value v -> 
+      substitution v x e e' ->
+      (E_App (E_Fun x t e) v) --> e'
   | ST_App_Left : 
-      ∀ (e₁ e₁' e₂ : expr),
-      e₁ --> e₁' ->
-      <{e₁ e₂}> --> <{e₁' e₂}>
-
+      ∀ (e1 e1' e2 : expr),
+      e1 --> e1' ->
+      (E_App e1 e2) --> (E_App e1' e2)
   | ST_App_Right : 
-      ∀ (v e e' : expr),
+      ∀ (v1 e2 e2' : expr),
+      value v1 ->
+      e2 --> e2' ->
+      (E_App v1 e2) --> (E_App v1 e2')
+  | ST_App_Exn_Left :
+      ∀ (exn : exception) (e : expr),
+      E_App (E_Exception exn) e --> (E_Exception exn)
+  | ST_App_Exn_Right :
+      ∀ (exn : exception) (v : expr),
       value v ->
-      e --> e' ->
-      <{v e}> --> <{v e'}>
+      E_App v (E_Exception exn) --> E_App v (E_Exception exn)
 
   | ST_If_True : 
-      ∀ (e₁ e₂ : expr),
-      <{if true then e₁ else e₂}> --> e₁
-      
+      ∀ (e1 e2 : expr),
+      (E_If E_True e1 e2) --> e1
   | ST_If_False : 
-      ∀ (e₁ e₂ : expr),
-      <{if false then e₁ else e₂}> --> e₂
-
+      ∀ (e1 e2 : expr),
+      (E_If E_False e1 e2) --> e2
   | ST_If : 
-      ∀ (e₁ e₁' e₂ e₃ : expr),
-      e₁ --> e₁' ->
-      <{if e₁ then e₂ else e₃}> --> <{if e₁' then e₂ else e₃}>
+      ∀ (e1 e1' e2 e3 : expr),
+      e1 --> e1' ->
+      (E_If e1 e2 e3) --> (E_If e1' e2 e3)
+  | ST_If_Exn :
+    ∀ (exn : exception) (e_true e_false : expr),
+    <{if `E_Exception exn` then e_true else e_false}> --> (E_Exception exn)
 
 
   | ST_Let_Left : 
-      ∀ (x : string) (e₁ e₁' e₂ : expr),
-      e₁ --> e₁' ->
-      <{let x = e₁ in e₂}>  -->  <{let x = e₁' in e₂}> 
-
+      ∀ (x : string) (e1 e1' e2 : expr),
+      e1 --> e1' ->
+      (E_Let x e1 e2) --> (E_Let x e1' e2)
   | ST_Let_Right : 
-      ∀ (x : string) (v e : expr),
-      value v ->
-      <{ let x = v in e }> --> sub v x e
+      ∀ (x : string) (v1 e2 e2' : expr),
+      value v1 ->
+      substitution v1 x e2 e2' ->
+      (E_Let x v1 e2) --> e2'
+  | ST_Let_Exn  :
+      ∀ (x : string) (exn : exception) (e : expr),
+      <{let x = `E_Exception exn` in e}> --> E_Exception exn
 
-  
+      
   | ST_Minus_Left :  
-      ∀ (e₁ e₁' e₂ : expr),
-      e₁ --> e₁' ->
-      <{ e₁ - e₂ }> --> <{ e₁' - e₂ }>
-
+      ∀ (e1 e1' e2 : expr),
+      e1 --> e1' ->
+      (E_Minus e1 e2) --> (E_Minus e1' e2)
   | ST_Minus_Right :  
-      ∀ (v e e' : expr),
-      value v ->
-      e --> e' ->
-      <{ v - e }> --> <{ v - e'}>
-
+      ∀ (v1 e2 e2' : expr),
+      value v1 ->
+      e2 --> e2' ->
+      (E_Minus v1 e2) --> (E_Minus v1 e2')
   | ST_Minus_Num : 
-      ∀ (z₁ z₂ : Z),
-      <{ z₁ - z₂ }> --> <{ `z₁ - z₂` }>
-  
+      ∀ (z1 z2 : Z),
+      (E_Minus (E_Num z1) (E_Num z2)) --> (E_Num (z1 - z2))
+  | ST_Minus_Left_Exn :
+      ∀ (exn : exception) (e : expr),
+      <{ `E_Exception exn` - e }> --> E_Exception exn 
+  | ST_Minus_Right_Exn :
+      ∀ (exn : exception) (v : expr),
+      value v ->
+      <{ v - `E_Exception exn` }> --> E_Exception exn
 
   | ST_Eq_Left :  
-      ∀ (e₁ e₁' e₂ : expr),
-      e₁ --> e₁' ->
-      <{ e₁ == e₂ }> --> <{ e₁' == e₂ }>
-
+      ∀ (e1 e1' e2 : expr),
+      e1 --> e1' ->
+      (E_Eq e1 e2) --> (E_Eq e1' e2)
   | ST_Eq_Right :  
-      ∀ (v e e' : expr),
-      value v ->
-      e --> e' ->
-      <{ v == e }> --> <{ v == e' }>
-
+      ∀ (v1 e2 e2' : expr),
+      value v1 ->
+      e2 --> e2' ->
+      (E_Eq v1 e2) --> (E_Eq v1 e2')
   | ST_Eq_Num_Eq : 
       ∀ (z : Z),
-      <{ z == z }> --> <{ true }>
-
+      (E_Eq (E_Num z) (E_Num z)) --> (E_True)
   | ST_Eq_Num_Neq : 
-      ∀ (z₁ z₂ : Z),
-      z₁ <> z₂ ->
-      <{ z₁ == z₂ }> --> <{ false }>
-
+      ∀ (z1 z2 : Z),
+      z1 <> z2 ->
+      (E_Eq (E_Num z1) (E_Num z2)) --> (E_False)
+  | ST_Eq_Left_Exn :
+      ∀ (exn : exception) (e : expr),
+      <{ `E_Exception exn` == e }> --> E_Exception exn 
+  | ST_Eq_Right_Exn :
+      ∀ (exn : exception) (v : expr),
+      value v ->
+      <{ v == `E_Exception exn` }> --> E_Exception exn
 
   | ST_Pair_Left :  
-      ∀ (e₁ e₁' e₂ : expr),
-      e₁ --> e₁' ->
-      <{ (e₁, e₂) }> --> <{ (e₁', e₂) }> 
-
+      ∀ (e1 e1' e2 : expr),
+      e1 --> e1' ->
+      (E_Pair e1 e2) --> (E_Pair e1' e2)
   | ST_Pair_Right :  
-      ∀ (v e e' : expr),
+      ∀ (v1 e2 e2' : expr),
+      value v1 ->
+      e2 --> e2' ->
+      (E_Pair v1 e2) --> (E_Pair v1 e2')
+  | ST_Pair_Left_Exn :
+      ∀ (exn : exception) (e : expr),
+      <{ (`E_Exception exn`, e) }> --> E_Exception exn 
+  | ST_Pair_Right_Exn :
+      ∀ (exn : exception) (v : expr),
       value v ->
-      e --> e' ->
-      <{ (v, e) }> --> <{ (v, e') }> 
+      <{ (v, `E_Exception exn`) }> --> E_Exception exn
+
 
   | ST_First :  
       ∀ (e e' : expr),
       e --> e' ->
-      <{first e}> --> <{first e'}>
-
+      (E_First e) --> (E_First e')
   | ST_First_Pair :  
       ∀ (v₁ v₂ : expr),
       value v₁ -> 
       value v₂ ->
-      <{first (v₁, v₂)}> --> v₁
+      (E_First (E_Pair v₁ v₂)) --> v₁
+  | ST_First_Exn :
+      ∀ (exn : exception),
+      <{first `E_Exception exn`}> --> E_Exception exn
 
   | ST_Second :  
       ∀ (e e' : expr),
       e --> e' ->
-      <{second e}> --> <{second e'}>
-
+      (E_Second e) --> (E_Second e')
   | ST_Second_Pair :  
       ∀ (v₁ v₂ : expr),
       value v₁ -> 
       value v₂ ->
-      <{second (v₁, v₂)}> --> v₂
+      (E_Second (E_Pair v₁ v₂)) --> v₂
+  | ST_Second_Exn :
+      ∀ (exn : exception),
+      <{second `E_Exception exn`}> --> E_Exception exn
 
+  | ST_Record_Tail : 
+      ∀ x e tail tail', 
+      blocking_expr e -> 
+      tail --> tail' -> 
+      (E_Record_Cons x e tail) --> (E_Record_Cons x e tail')
   
-  | ST_Records : 
-      ∀ (rec rec': lsexpr),
-      rec -->ₗ rec' -> 
-      <{ { rec } }> --> <{ { rec' } }>
-
-  | ST_Access : 
-      ∀ (x : string) (e e' : expr),
+  | ST_Record_Cons : 
+      ∀ x e e' tail,
       e --> e' -> 
-      <{ e::x }> --> <{ e'::x }>
+      (E_Record_Cons x e tail) --> (E_Record_Cons x e' tail)      
+  
+  | ST_Access : 
+      ∀ x e e',
+      e --> e' ->
+      (E_Record_Access e x) --> (E_Record_Access e' x)
 
   | ST_Access_Value : 
       ∀ x e e',
-      value_lsexpr e -> 
-      lookup_lsexpr x e = Some e' ->
-      <{ { e }::x }> --> e'
+      blocking_expr e -> 
+      lookup_val_record x e = Some e' ->
+      (E_Record_Access e x) --> e'
 
-  
   | ST_Fix :
       ∀ (e e': expr),
       e --> e' ->
-      <{ fix e }> --> <{ fix e' }>
+      (E_Fix e) --> (E_Fix e')
   
   | ST_Fix_Fun :
-      ∀ (x : string) (t : type) (e : expr),
-      <{ fix (fun x : t => e) }> --> sub <{ fix (fun x : t => e)}> x e
-  
+      ∀ x t e e',
+      substitution (E_Fix (E_Fun x t e)) x e e' ->
+      (E_Fix (E_Fun x t e)) --> e'
+  | ST_Fix_Exn :
+      ∀ (exn : exception) (e : expr),
+      <{fix `E_Exception exn`}> --> E_Exception exn
 
   | ST_In_Left :
-      ∀ (t₁ t₂ : type) (e e' : expr), 
+      ∀ t₁ t₂ e e', 
       e --> e' -> 
-      <{ inl <t₁ | t₂> e }> --> <{ inl <t₁ | t₂> e' }>
+      E_In_Left t₁ t₂ e --> E_In_Left t₁ t₂ e'
 
   | ST_In_Right :
-      ∀ (t₁ t₂ : type) (e e' : expr), 
+      ∀ t₁ t₂ e e', 
       e --> e' -> 
-      <{ inr <t₁ | t₂> e }> --> <{ inr <t₁ | t₂> e' }>
+      E_In_Right t₁ t₂ e --> E_In_Right t₁ t₂ e'
   
   | ST_Match_Main :
-      ∀ (e e' eₗ eᵣ : expr),
+      ∀ e e' e_left e_right,
       e --> e' ->
-      <{ match e with | inl => eₗ | inr =>  eᵣ end }> --> 
-      <{ match e' with | inl => eₗ | inr =>  eᵣ end }>
+      E_Match e e_left e_right --> E_Match e' e_left e_right
+
 
   | ST_Match_Left :
-      ∀ (v eₗ eₗ' eᵣ : expr),
-      value v ->
-      eₗ --> eₗ' -> 
-      <{ match v with | inl => eₗ | inr =>  eᵣ end }> --> 
-      <{ match v with | inl => eₗ' | inr =>  eᵣ end }>
+      ∀ e e_left e_left' e_right,
+      value e ->
+      e_left --> e_left' -> 
+      E_Match e e_left e_right --> E_Match e e_left' e_right
 
   | ST_Match_Right :
-      ∀ (v vₗ eᵣ eᵣ' : expr),
-      value v ->
-      value vₗ ->
-      eᵣ --> eᵣ' -> 
-      <{ match v with | inl => vₗ | inr =>  eᵣ end }> --> 
-      <{ match v with | inl => vₗ | inr =>  eᵣ' end }>
+      ∀ e e_left e_right e_right',
+      value e -> 
+      value e_left -> 
+      e_right --> e_right' -> 
+      E_Match e e_left e_right --> E_Match e e_left e_right'
 
   | ST_Match_Left_App :
-      ∀ (t₁ t₂ : type) (v vₗ vᵣ : expr),
-      value v ->
-      value vₗ ->
-      value vᵣ ->
-      <{ match inl <t₁ | t₂> v with | inl => vₗ | inr =>  vᵣ end }> --> 
-      <{vₗ v}>
+      ∀ t₁ t₂ e e_left e_right,
+      value e -> 
+      value e_left -> 
+      value e_right -> 
+      E_Match (E_In_Left t₁ t₂ e) e_left e_right --> E_App e_left e
 
   | ST_Match_Right_App :
-    ∀ (t₁ t₂ : type) (v vₗ vᵣ : expr),
-      value v ->
-      value vₗ ->
-      value vᵣ ->
-      <{ match inr <t₁ | t₂> v with | inl => vₗ | inr =>  vᵣ end }> --> 
-      <{vᵣ v}>
-  
+    ∀ t₁ t₂ e e_left e_right,
+    value e -> 
+    value e_left -> 
+    value e_right -> 
+    E_Match (E_In_Right t₁ t₂ e) e_left e_right --> E_App e_right e
+
   | ST_Sum_Constr :
-      ∀ (constr : string) (e e' : expr),
+      ∀ constr e e',
       e --> e' -> 
       E_Sum_Constr constr e --> E_Sum_Constr constr e'
+  | ST_Sum_Constr_Exn :
+      ∀ constr exn,
+      E_Sum_Constr constr (E_Exception exn) --> E_Exception exn
 
   | ST_Sum_Match_Main : 
-      ∀ (e e' default : expr) (branches : lsexpr), 
+      ∀ e e' branches, 
       e --> e' -> 
-      <{match_sum e  with branches : default end_sum }> --> 
-      <{match_sum e' with branches : default end_sum }>
-
+      (E_Sum_Match e branches) --> (E_Sum_Match e' branches)
+  | ST_Sum_Match_Main_Exn : 
+      ∀ exn branches, 
+      (E_Sum_Match (E_Exception exn) branches) --> E_Exception exn
   | ST_Sum_Match :
-      ∀ (v default : expr) (branches branches' : lsexpr), 
+      ∀ v branches branches', 
       value v -> 
       branches -->ₗ branches' ->
-      <{match_sum v with branches  : default end_sum }> --> 
-      <{match_sum v with branches' : default end_sum }>
-  
-  | ST_Sum_Match_Default :
-      ∀ (v default default' : expr) (branches : lsexpr), 
-      value v -> 
-      value_lsexpr branches ->
-      default --> default' ->
-      <{match_sum v with branches : default  end_sum }> --> 
-      <{match_sum v with branches : default' end_sum }>
-
+      (E_Sum_Match v branches) 
+      --> (E_Sum_Match v branches')
   | ST_Sum_Match_Apply :
-      ∀ (constr : string) (v b default: expr) (branches : lsexpr), 
+      ∀ constr v branches b, 
       value v -> 
       value_lsexpr branches ->
-      value default -> 
-      lookup_lsexpr constr branches = Some b ->
-      <{match_sum `E_Sum_Constr constr v` with branches : default end_sum }> 
+      lookup_constr constr branches = Some b ->
+      (E_Sum_Match 
+        (E_Sum_Constr constr v)
+        branches
+      ) 
       --> <{b v}>
   | ST_Sum_Match_Apply_Not_Found :
-      ∀ (constr : string) (v default: expr) (branches : lsexpr), 
+      ∀ constr v branches b, 
       value v -> 
       value_lsexpr branches ->
-      value default -> 
-      lookup_lsexpr constr branches = None ->
-      <{match_sum `E_Sum_Constr constr v` with branches : default end_sum }> 
-      --> default
-where
-  "x --> y" := (step x y)
-with 
-  step_lsexpr : lsexpr -> lsexpr -> Prop := 
-    | ST_LSExpr_Cons :
-        ∀ (x : string) (e e' : expr) (tail : lsexpr),
-        e --> e' -> 
-        <{ x := e ; tail}> -->ₗ <{ x := e' ; tail}>
+      lookup_constr constr branches = None ->
+      (E_Sum_Match 
+        (E_Sum_Constr constr v)
+        branches
+      ) 
+      --> E_Exception Ex_Unhandled_Case
 
-    | ST_LSExpr_Tail :
-        ∀ (x : string) (v : expr) (tail tail' : lsexpr),
-        value v -> 
-        tail -->ₗ tail' ->
-        <{ x := v ; tail}> -->ₗ <{ x := v ; tail'}>
+where
+    "x --> y" := (step x y)
+     
+with step_lsexpr : lsexpr -> lsexpr -> Prop := 
+  | ST_LSExpr_Cons :
+      ∀ constr e e' branches,
+      e --> e' -> 
+      step_lsexpr 
+        (LSE_Cons constr e branches) 
+        (LSE_Cons constr e' branches)
+  | ST_LSExpr_Tail :
+      ∀ constr v branches branches',
+      blocking_expr v -> 
+      branches -->ₗ branches' ->
+      (LSE_Cons constr v branches) -->ₗ (LSE_Cons constr v branches') 
 where 
     "x -->ₗ y" := (step_lsexpr x y)
 .
 
-Check ∀ (z₁ z₂ : Z),
-      <{ z₁ - z₂ }> --> <{ `z₁ - z₂` }>.
-
 Hint Constructors step : local_hints.
 Hint Constructors step_lsexpr : local_hints.
+
+
 
 Local Lemma not_value: 
   ∀ e e',
@@ -285,12 +317,15 @@ Proof with eauto with local_hints.
   apply expr_mut_ind with (P := P) (P0 := P0); unfold P; unfold P0;
   clear P P0;
   try (
-    intros * IH1 * IH2 * IH3 * H_val H_contra;
+    intros * H_val H_contra;
+    inversion H_contra;
+    fail
+  );
+  try (
+    intros * IH * H_val H_contra;
     inversion H_val;
     inversion H_contra; subst;
-    try (eapply IH1; eauto with local_hints; fail);
-    try (eapply IH2; eauto with local_hints; fail);
-    try (eapply IH3; eauto with local_hints; fail);
+    try (eapply IH; eauto with local_hints; fail);
     fail
   );
   try (
@@ -302,19 +337,17 @@ Proof with eauto with local_hints.
     fail
   );
   try (
-    intros * IH * H_val H_contra;
+    intros * IH1 * IH2 * IH3 * H_val H_contra;
     inversion H_val;
     inversion H_contra; subst;
-    try (eapply IH; eauto with local_hints; fail);
-    fail
-  );
-  try (
-    intros * H_val H_contra;
-    inversion H_contra;
+    try (eapply IH1; eauto with local_hints; fail);
+    try (eapply IH2; eauto with local_hints; fail);
+    try (eapply IH3; eauto with local_hints; fail);
     fail
   ).
 Qed.
 Hint Resolve not_value : local_hints.
+
 
 Local Lemma not_value_lsexpr :
   ∀ branches branches', 
@@ -373,26 +406,26 @@ Proof with eauto with local_hints.
     intros * IH1 * IH2 * H_st1 H_st2;
     inversion H_st1; subst;
     inversion H_st2; subst;
-    try (simpl in *; eauto with local_hints; fail);
+    try (eapply Subst.deterministic; eauto with local_hints; fail);
     try (f_equal; eauto with local_hints; fail);
     try (exfalso; eapply not_value; eauto with local_hints; fail);
     fail
   ).
   - intros * IH1 * IH2 * H_st1 H_st2.
     inversion H_st1; subst.
-    + inversion H_st2; subst...
-      inversion H3.
-      exfalso; eapply not_value with (e:=e2)...
+    + inversion H_st2; subst.
+      * eapply Subst.deterministic...
+      * inversion H4.
+      * eapply not_value in H5... contradiction.
     + inversion H_st1; subst; 
       try (
-        inversion H_st2; subst;try (simpl in *; eauto with local_hints; fail); 
+        inversion H_st2; subst;try (eapply Subst.deterministic; eauto with local_hints; fail); 
         try (inversion H0; fail);
         f_equal; eauto with local_hints;
         try (exfalso; eapply not_value; eauto with local_hints; fail);
         fail
       ).
-      inversion H2.
-    + inversion H_st2; subst;
+    + inversion H_st2; subst; 
       try (exfalso; eapply not_value; eauto with local_hints; fail).
       f_equal...
   - intros * IH1 * IH2 * IH3 * H_st1 H_st2.
@@ -459,15 +492,16 @@ Proof with eauto with local_hints.
     inversion H_st1;
     inversion H_st2; subst.
     + f_equal... 
-    + exfalso; eapply not_value with (e:=<{ { e2 } }>)...
-    + exfalso; eapply not_value with (e:=<{ { e1 } }>)... 
-    + inversion H4. rewrite H0 in *. rewrite H3 in H8. inversion H8...  
+    + exfalso; eapply not_value; eauto with local_hints. 
+    + exfalso; eapply not_value; eauto with local_hints. 
+    + rewrite H3 in H8. inversion H8...  
   - intros * IH * H_st1 H_st2.
     inversion H_st1; subst;
     inversion H_st2; subst;
     try (f_equal; eauto with local_hints).
     + inversion H0.
-    + inversion H0.
+    + inversion H1.
+    + eapply Subst.deterministic... 
   - intros * IH1 * IH2 * IH3 * H_st1 H_st2.
     inversion H_st1; subst.
     + inversion H_st2; subst.
@@ -475,9 +509,9 @@ Proof with eauto with local_hints.
       * exfalso; eapply not_value; eauto with local_hints.
       * exfalso; eapply not_value with (e:= e0); eauto with local_hints.
       * inversion H3; subst. 
-        exfalso; eapply not_value with (e:= v); eauto with local_hints.
+        exfalso; eapply not_value with (e:= e1); eauto with local_hints.
       * inversion H3; subst. 
-        exfalso; eapply not_value with (e:= v); eauto with local_hints.
+        exfalso; eapply not_value with (e:= e1); eauto with local_hints.
     + inversion H_st2; subst.
       * exfalso; eapply not_value; eauto with local_hints.
       * f_equal...
@@ -490,42 +524,27 @@ Proof with eauto with local_hints.
       * f_equal...
       * exfalso; eapply not_value; eauto with local_hints.
       * exfalso; eapply not_value; eauto with local_hints.
-    + inversion H_st2; subst...
-      * inversion H6; subst. 
-        exfalso; eapply not_value with (e := v)...
-      * exfalso; eapply not_value with (e := case_left)...
-      * exfalso; eapply not_value with (e := case_right)...
-        
-    + inversion H_st2; subst...
-      * inversion H6; subst. 
-        exfalso; eapply not_value with (e := v)...
-      * exfalso; eapply not_value with (e := case_left)...
-      * exfalso; eapply not_value with (e := case_right)...
-  - intros * IH1 * IH2 * IH3 * H_st1 H_st2.
-    inversion H_st1; subst.
-    + inversion H_st2; subst; try (f_equal; eauto with local_hints; fail);
-      try (exfalso; eapply not_value; eauto with local_hints; fail);
-      try (
-          inversion H3; 
-          exfalso; eapply not_value with (e := v); eauto with local_hints).
-    + inversion H_st2; subst; try (f_equal; eauto with local_hints; fail);
-      try (exfalso; eapply not_value; eauto with local_hints; fail);
-      try (exfalso; eapply not_value_lsexpr; eauto with local_hints; fail).
-    + inversion H_st2; subst; try (f_equal; eauto with local_hints; fail);
-      try (exfalso; eapply not_value; eauto with local_hints; fail);
-      try (exfalso; eapply not_value_lsexpr; eauto with local_hints; fail).
     + inversion H_st2; subst.
-      * inversion H7; subst.
-        exfalso; eapply not_value with (e:=v)...
-      * inversion H7; subst.
-        exfalso; eapply not_value_lsexpr...
-      * exfalso; eapply not_value with (e:=default)...
-      * rewrite H6 in H11. inversion H11. f_equal...
-      * rewrite H6 in H11. inversion H11. 
-    + inversion H_st2; subst; try (f_equal; eauto with local_hints; fail);
-      try (exfalso; eapply not_value_lsexpr; eauto with local_hints; fail).
-      * inversion H7; subst.
-        exfalso; eapply not_value with(e:=v)...
-      * exfalso; eapply not_value with (e:=e'₁)...
-      * rewrite H6 in H11; inversion H11.
+      * inversion H6; subst. 
+        exfalso; eapply not_value with (e := e1)...
+      * exfalso; eapply not_value with (e := case_left)...
+      * exfalso; eapply not_value with (e := case_right)...
+      * eauto.
+        
+    + inversion H_st2; subst.
+      * inversion H6; subst. 
+        exfalso; eapply not_value with (e := e1)...
+      * exfalso; eapply not_value with (e := case_left)...
+      * exfalso; eapply not_value with (e := case_right)...
+      * eauto.
+  - intros * IH1 * IH2 * H_st1 H_st2.
+    inversion H_st1; inversion H_st2; subst; 
+    try (exfalso; eapply not_value; eauto with local_hints; fail);
+    try (exfalso; eapply not_value_lsexpr; eauto with local_hints; fail).
+    + apply (IH1 _ _ H2) in H6; subst...
+    + inversion H2. exfalso; eapply not_value... 
+    + apply (IH2 _ _ H3) in H8; subst...
+    + inversion H8; subst...
+      exfalso; eapply not_value...
+    + inversion H5; f_equal; subst;rewrite H4 in H10; inversion H10... 
 Qed.
