to_rewrite/okay/Closed.v
@@ -1,0 +1,519 @@
+From Coq Require Import Unicode.Utf8.
+From Coq Require Import Strings.String.
+Local Open Scope Z_scope.
+Require Import ZArith.
+Require Import Hints.
+Require Import Syntax.
+Require Import Types.
+Require Maps.
+Import Maps.Notations.
+Require Import List.
+Import ListNotations.
+
+(* TODO: Branches des matchs *)
+Inductive is_free_in (x : string) : expr -> Prop :=
+  | Free_Var : is_free_in x <{x}>
+  | Free_App_Left : 
+      ∀ e₁ e₂, 
+      is_free_in x e₁ -> 
+      is_free_in x <{e₁ e₂}>
+  | Free_App_Right : 
+      ∀ e₁ e₂, 
+      is_free_in x e₂ -> 
+      is_free_in x <{e₁ e₂}>
+  | Free_Fun : 
+      ∀ y t e, 
+      y <> x -> 
+      is_free_in x e -> 
+      is_free_in x <{fun y : t => e}> 
+  | Free_If_Cond : 
+      ∀ e₁ e₂ e₃, 
+      is_free_in x e₁ -> 
+      is_free_in x <{if e₁ then e₂ else e₃}> 
+  | Free_If_Left : 
+      ∀ e₁ e₂ e₃, 
+      is_free_in x e₂ -> 
+      is_free_in x <{if e₁ then e₂ else e₃}> 
+  | Free_If_Right : 
+      ∀ e₁ e₂ e₃, 
+      is_free_in x e₃ -> 
+      is_free_in x <{if e₁ then e₂ else e₃}> 
+  | Free_Let_Left : 
+      ∀ y e₁ e₂, 
+      is_free_in x e₁ -> 
+      is_free_in x <{let y = e₁ in e₂}>
+  | Free_Let_Right : 
+      ∀ y e₁ e₂, 
+      y <> x -> is_free_in x e₂ -> 
+      is_free_in x <{let y = e₁ in e₂}>
+  | Free_Minus_Left : 
+      ∀ e₁ e₂, 
+      is_free_in x e₁ -> 
+      is_free_in x <{e₁ - e₂}>
+  | Free_Minus_Right : 
+      ∀ e₁ e₂, 
+      is_free_in x e₂ -> 
+      is_free_in x <{e₁ - e₂}>
+
+  | Free_Eq_Left : 
+      ∀ e₁ e₂, 
+      is_free_in x e₁ -> 
+      is_free_in x <{e₁ == e₂}>
+  | Free_Eq_Right : 
+      ∀ e₁ e₂, 
+      is_free_in x e₂ -> 
+      is_free_in x <{e₁ == e₂}>
+  | Free_Pair_Left : 
+      ∀ e₁ e₂, 
+      is_free_in x e₁ -> 
+      is_free_in x (E_Pair e₁ e₂) 
+  | Free_Pair_Right : 
+      ∀ e₁ e₂, 
+      is_free_in x e₂ -> 
+      is_free_in x (E_Pair e₁ e₂) 
+  | Free_First : 
+    ∀ e, 
+    is_free_in x e -> 
+    is_free_in x (E_First e)
+  | Free_Second : 
+    ∀ e, 
+    is_free_in x e -> 
+    is_free_in x (E_Second e)
+
+  | Free_Record_Cons_tail :
+    ∀ y e tail, 
+    is_free_in x tail -> 
+    is_free_in x (E_Record_Cons y e tail)
+  | Free_Record_Cons_head :
+    ∀ y e tail, 
+    is_free_in x e -> 
+    is_free_in x (E_Record_Cons y e tail)
+
+  | Free_Record_Access :
+    ∀ y e, 
+      is_free_in x e -> 
+      is_free_in x (E_Record_Access e y) 
+
+  | Free_Fix :  
+      ∀ e, 
+      is_free_in x e -> 
+      is_free_in x (E_Fix e) 
+
+  | Free_In_Left :
+      ∀ e t₁ t₂, 
+      is_free_in x e ->
+      is_free_in x (E_In_Left t₁ t₂ e)
+  
+  | Free_In_Right :
+      ∀ e t₁ t₂, 
+      is_free_in x e -> 
+      is_free_in x (E_In_Right t₁ t₂ e)
+
+  | Free_Match_Main :
+      ∀ e e_left e_right, 
+      is_free_in x e -> 
+      is_free_in x (E_Match e e_left e_right)
+
+  | Free_Match_Left :
+      ∀ e e_left e_right, 
+      is_free_in x e_left -> 
+      is_free_in x (E_Match e e_left e_right)
+  
+  | Free_Match_Right :
+      ∀ e e_left e_right, 
+      is_free_in x e_right -> 
+      is_free_in x (E_Match e e_left e_right)
+  | Free_Sum_Constr :
+      ∀ e constr, 
+      is_free_in x e -> 
+      is_free_in x (E_Sum_Constr constr e)
+  
+  | Free_Sum_Match_Base :
+    ∀ e branches, 
+    is_free_in x e -> 
+    is_free_in x (E_Sum_Match e branches)
+
+  | Free_Sum_Match_Rec_Branches :
+    ∀ e branches,
+    is_free_in_lsexpr x branches -> 
+    is_free_in x (E_Sum_Match e branches)
+
+
+with is_free_in_lsexpr  (x : string) : lsexpr -> Prop :=
+  | Free_LSExpr_Cons :
+    ∀ e constr tail,
+    is_free_in x e -> 
+    is_free_in_lsexpr x (LSE_Cons constr e tail)
+  | Free_LSExpr_Tail :
+    ∀ e constr tail,
+    is_free_in_lsexpr x tail -> 
+    is_free_in_lsexpr x (LSE_Cons constr e tail)
+.
+
+Hint Constructors is_free_in : local_hints.
+Hint Constructors is_free_in_lsexpr : local_hints.
+
+Definition closed e := ∀ x, ¬ is_free_in x e.
+Definition closed_lsexpr e := ∀ x, ¬ is_free_in_lsexpr x e.
+
+Hint Unfold closed : local_hints.
+Hint Unfold closed_lsexpr : local_hints.
+
+Lemma free_has_type :
+    ∀ e, ∀ Γ Σ t x,
+    is_free_in x e ->
+    has_type Σ Γ e t ->  
+    ∃ t_x, Γ ? x = Some t_x.
+Proof with eauto with local_hints.
+  pose (
+    P (e : expr) := 
+      ∀ Γ Σ t x,
+      is_free_in x e ->
+      has_type Σ Γ e t ->  
+      ∃ t_x, Γ ? x = Some t_x
+  ). 
+  pose (
+    P0 (branches : lsexpr) :=
+      ∀ Γ Σ name_sum t x,
+        is_free_in_lsexpr x branches ->
+        has_type_lsexpr name_sum Σ Γ branches t ->  
+        ∃ t_x, Γ ? x = Some t_x
+  ).
+  intro.
+  apply expr_mut_ind with (P := P) (P0 := P0); 
+  unfold P; unfold P0; intros;
+  try (try inversion H; try inversion H0; try inversion H1; try inversion H2; try inversion H3; subst; eauto with local_hints; fail).
+  - inversion H0; 
+    inversion H1;
+    subst.
+    eapply H with (Σ := Σ) (Γ := (x |-> t; Γ)) in H6...
+    destruct H6 as [t_x Ht_x].
+    exists t_x.
+    rewrite <- Ht_x.
+    rewrite Maps.update_neq...
+  - inversion H1; 
+    inversion H2;
+    subst.
+    + eapply H with (Σ := Σ) (Γ := Γ) in H4...
+    + eapply H0 with (Σ := Σ) (Γ := (x |-> t1; Γ)) in H7...
+      destruct H7 as [t_x Ht_x].
+      exists t_x.
+      rewrite <- Ht_x.
+      rewrite Maps.update_neq...
+Qed.
+
+Hint Resolve free_has_type : local_hints.
+
+
+Theorem typed_empty :
+    ∀ e, ∀ Σ t,
+    has_type Σ empty e t ->  
+    closed e.
+Proof with eauto with local_hints.
+  pose (
+    P (e : expr) := 
+      ∀ Σ t,
+      has_type Σ empty e t ->  
+      closed e
+  ).
+  pose (
+    P0 (branches : lsexpr) :=
+      ∀ name_sum Σ t,
+        has_type_lsexpr name_sum Σ empty branches t ->  
+        closed_lsexpr branches
+  ).
+  intro e.
+  apply expr_mut_ind with (P := P) (P0 := P0);
+  unfold P; unfold P0; intros; intros x_contra H_contra;
+  try (inversion H_contra; fail).
+  - inversion H. inversion H3.
+  - inversion H1; subst. 
+    inversion H_contra; subst.
+    + eapply (H _ _ H8)...
+    + eapply (H0 _ _ H6)...
+  - inversion H_contra; inversion H0; subst.
+    eapply free_has_type in H_contra as [t_x H_eq]...
+    inversion H_eq.
+  - inversion H_contra; inversion H2; subst.
+    + eapply H in H4...        
+    + eapply H0 in H4...        
+    + eapply H1 in H4...
+  - inversion H_contra; inversion H1; subst.
+    + eapply (H _ _ H12)...
+    + eapply free_has_type in H_contra as [t_x H_eq]...
+      inversion H_eq.
+  - inversion H_contra; inversion H1; subst.
+    + eapply (H _ _ H9)...
+    + eapply (H0 _ _ H11)...
+  - inversion H_contra; inversion H1; subst.
+    + eapply (H _ _ H9)...
+    + eapply (H0 _ _ H11)...
+  - inversion H_contra; inversion H1; subst.
+    + eapply (H _ _ H9)...
+    + eapply (H0 _ _ H11)...
+  - inversion H_contra; inversion H0; subst.
+    eapply (H _ _ H6)...
+  - inversion H_contra; inversion H0; subst.
+    eapply (H _ _ H6)...
+  - inversion H_contra; inversion H1; subst.
+    + eapply (H0 _ _ H13)...
+    + eapply (H _ _ H11)...
+  - inversion H_contra; inversion H0; subst.
+    eapply (H _ _ H8)...
+  - inversion H_contra; inversion H0; subst.
+    eapply (H _ _ H6)...
+  - inversion H_contra; inversion H0; subst.
+    eapply (H _ _ H11)...
+  - inversion H_contra; inversion H0; subst.
+    eapply (H _ _ H11)...
+  - inversion H_contra; inversion H2; subst.
+    + eapply (H _ _ H12)...
+    + eapply (H0 _ _ H14)...
+    + eapply (H1 _ _ H15)...
+  - inversion H_contra; inversion H0; subst.
+    eapply (H _ _ H10)...
+  - inversion H_contra; inversion H1; subst.
+    + eapply (H _ _ H9)...
+    + apply H0 in H11.
+      eapply H11...
+  - inversion H_contra; inversion H1; subst.
+    + eapply (H _ _ H15)...
+    + apply H0 in H12. eapply H12... 
+Qed.
+  
+Hint Resolve typed_empty : local_hints.
+
+
+Lemma closed_app : 
+  ∀ e₁ e₂, 
+  closed (E_App e₁ e₂) -> 
+  closed e₁ /\ closed e₂.
+Proof.
+  intros.
+  unfold closed in *.
+  split; 
+    intros x H_contra;
+    apply H with x;
+    eauto with local_hints.
+Qed.
+
+Hint Resolve closed_app : local_hints.
+
+
+
+Lemma closed_let : 
+  ∀ x e₁ e₂, 
+  closed (E_Let x e₁ e₂) -> 
+  closed e₁.
+Proof.
+  intros.
+  unfold closed in *.
+  intros x' H_contra.
+  apply H with x'.
+  eauto with local_hints.
+Qed.
+
+Hint Resolve closed_let : local_hints.
+
+
+Lemma closed_if : 
+  ∀ e₁ e₂ e₃, 
+  closed (E_If e₁ e₂ e₃) -> 
+  closed e₁ /\ closed e₂ /\ closed e₃.
+Proof.
+  intros.
+  unfold closed in *.
+  repeat split;
+    intros x H_contra;
+    apply H with x;
+    eauto with local_hints.
+Qed.
+
+Hint Resolve closed_if : local_hints.
+
+
+Lemma closed_minus : 
+  ∀ e₁ e₂, 
+  closed (E_Minus e₁ e₂) -> 
+  closed e₁ /\ closed e₂.
+Proof.
+  intros.
+  unfold closed in *.
+  split; 
+    intros x H_contra;
+    apply H with x;
+    eauto with local_hints.
+Qed.
+
+Hint Resolve closed_minus : local_hints.
+
+Lemma closed_eq : 
+  ∀ e₁ e₂, 
+  closed (E_Eq e₁ e₂) -> 
+  closed e₁ /\ closed e₂.
+Proof.
+  intros.
+  unfold closed in *.
+  split; 
+    intros x H_contra;
+    apply H with x;
+    eauto with local_hints.
+Qed.
+
+Hint Resolve closed_eq : local_hints.
+
+Lemma closed_pair : 
+  ∀ e₁ e₂, 
+  closed (E_Pair e₁ e₂) -> 
+  closed e₁ /\ closed e₂.
+Proof.
+  intros.
+  unfold closed in *.
+  split; 
+    intros x H_contra;
+    apply H with x;
+    eauto with local_hints.
+Qed.
+
+Hint Resolve closed_pair : local_hints.
+
+Lemma closed_first : 
+  ∀ e, 
+  closed (E_First e) -> 
+  closed e.
+Proof.
+  intros.
+  unfold closed in *.
+  intros x' H_contra;
+  apply H with x';
+  eauto with local_hints.
+Qed.
+Hint Resolve closed_first : local_hints.
+
+
+
+Lemma closed_second : 
+  ∀ e, 
+  closed (E_Second e) -> 
+  closed e.
+Proof.
+  intros.
+  unfold closed in *.
+  intros x' H_contra;
+  apply H with x';
+  eauto with local_hints.
+Qed.
+Hint Resolve closed_second : local_hints.
+
+
+Lemma closed_record : 
+  ∀ x e₁ e₂, 
+  closed (E_Record_Cons x e₁ e₂) -> 
+  closed e₁ /\ closed e₂.
+Proof.
+  intros.
+  unfold closed in *.
+  split; 
+    intros x' H_contra;
+    apply H with x';
+    eauto with local_hints.
+Qed.
+Hint Resolve closed_record : local_hints.
+
+
+Lemma closed_access : 
+  ∀ x e, 
+  closed (E_Record_Access e x) -> 
+  closed e.
+Proof.
+  intros.
+  unfold closed in *.
+  intros x' H_contra;
+  apply H with x';
+  eauto with local_hints.
+Qed.
+Hint Resolve closed_access : local_hints.
+
+
+Lemma closed_fix : 
+  ∀ e, 
+  closed (E_Fix e) -> 
+  closed e.
+Proof.
+  intros.
+  unfold closed in *.
+  intros x' H_contra;
+  apply H with x';
+  eauto with local_hints.
+Qed.
+Hint Resolve closed_fix : local_hints.
+
+
+Lemma closed_in_left :
+  ∀ e t₁ t₂,
+  closed (E_In_Left t₁ t₂ e) ->  
+  closed e.
+Proof.
+  intros.
+  unfold closed in *.
+  intros x' H_contra;
+  apply H with x';
+  eauto with local_hints.
+Qed.
+Hint Resolve closed_in_left : local_hints.
+
+Lemma closed_in_right :
+  ∀ e t₁ t₂,
+  closed (E_In_Right t₁ t₂ e) ->  
+  closed e.
+Proof.
+  intros.
+  unfold closed in *.
+  intros x' H_contra;
+  apply H with x';
+  eauto with local_hints.
+Qed.
+Hint Resolve closed_in_right : local_hints.
+
+
+
+Lemma closed_match :
+  ∀ e e_left e_right,
+  closed (E_Match e e_left e_right) -> 
+  closed e /\ closed e_left /\ closed e_right.
+Proof.
+  intros.
+  unfold closed in *.
+  repeat split;
+    intros x' H_contra;
+    apply H with x';
+    eauto with local_hints.
+Qed.
+Hint Resolve closed_match : local_hints.
+
+Lemma closed_sum_constr :
+  ∀ constr e,
+  closed (E_Sum_Constr constr e) -> 
+  closed e.
+Proof.
+  intros.
+  unfold closed in *.
+    intros x' H_contra;
+    apply H with x';
+    eauto with local_hints.
+Qed.
+Hint Resolve closed_sum_constr : local_hints.
+
+Lemma closed_sum_match : 
+  ∀ e branches, 
+  closed (E_Sum_Match e branches) -> 
+  closed e /\ closed_lsexpr branches.
+Proof.
+  intros.
+  unfold closed in *.
+  unfold closed_lsexpr in *.
+  split;
+    intros x H_contra;
+    apply H with x;
+    eauto with local_hints.
+Qed.
