to_rewrite/okay/Preservation.v
@@ -1,0 +1,124 @@
+From Coq Require Import Unicode.Utf8.
+From Coq Require Import Strings.String.
+Local Open Scope Z_scope.
+Require Import ZArith.
+Require Import Hints.
+Require Import Syntax.
+Require Import Types.
+Require Import Subst.
+Require Import Step.
+Require Import Canonical_form.
+Require Maps.
+Import Maps.Notations.
+
+Lemma test1 : 
+  ∀ Σ Γ constr v branches t s e,
+  has_type Σ Γ (E_Sum_Match (E_Sum_Constr constr v) (LSE_Cons s e branches)) t -> 
+  s ≠ constr -> 
+  has_type Σ Γ (E_Sum_Match (E_Sum_Constr constr v) branches) t.
+Proof. 
+  Admitted.
+
+
+Lemma test : 
+  ∀ Σ Γ constr v branches t b,
+  has_type Σ Γ (E_Sum_Match (E_Sum_Constr constr v) branches) t ->
+  lookup_constr constr branches = Some b ->
+  ∃ t_arg, 
+      has_type Σ Γ v t_arg 
+   /\ has_type Σ Γ b {{t_arg -> t}}.
+Proof.
+  intros.
+  induction branches.
+  - inversion H0.
+  - simpl in H0.
+    destruct (String.eqb_spec constr s); subst.
+    + admit.
+    + inversion H; subst. 
+  Admitted.
+  
+
+
+
+
+(* Lemma test: 
+  ∀ name_sum constr Σ Γ branches b t t_arg, 
+  lookup_type_sum constr Σ = Some (name_sum, t_arg) ->
+  lookup_constr constr branches = Some b ->
+  has_type_lsexpr name_sum Σ Γ branches t ->
+  has_type Σ Γ b {{t_arg -> t}}
+.
+Proof with eauto with local_hints.
+  intros.
+  induction branches.
+  - inversion H0.
+  - simpl in H0.
+    destruct (String.eqb_spec constr s); subst.
+    + inversion H0; subst.
+      inversion H1; subst. 
+      rewrite H in H10.
+      inversion H10; subst...
+    + inversion H1; subst. 
+      apply IHbranches...
+Qed. *)
+
+Theorem preservation : 
+  ∀ e Σ e' t,
+  has_type Σ empty e t  ->
+  e --> e'  ->
+  has_type Σ empty e' t.
+Proof with eauto 3 with local_hints.
+  intro e.
+  pose (
+    P (e: expr) :=
+      ∀ Σ e' t,
+        has_type Σ empty e t  ->
+        e --> e'  ->
+        has_type Σ empty e' t
+  ).
+  pose (
+    P0 (branches: lsexpr) :=
+      ∀ name_sum Σ branches' t,
+        has_type_lsexpr name_sum Σ empty branches t  ->
+        branches -->ₗ branches'  ->
+        has_type_lsexpr name_sum Σ empty branches' t
+  ).
+  apply expr_mut_ind with (P := P) (P0 := P0); unfold P; unfold P0;
+  clear P P0;
+  try (intros * IH1 * IH2 * IH3 * H_type H_step);
+  try (intros * IH1 * IH2 * H_type H_step);
+  try (intros * IH * H_type H_step);
+  try (intros * H_type H_step);
+  try (inversion H_step; fail);
+  try (inversion H_step; subst;
+    inversion H_type; subst; eauto 3 with local_hints; fail).
+  - inversion H_step; subst;
+    inversion H_type; subst; 
+    try (eapply T_App; eauto with local_hints; fail).
+    inversion H7; subst.
+    eapply Subst.preserves_typing...
+  - inversion H_step; subst;
+    inversion H_type; subst...
+    inversion H4...
+  - inversion H_step; subst;
+    inversion H_type; subst...
+    inversion H4...
+  - inversion H_step; subst.
+    + inversion H_type; subst.
+      apply T_Fix...
+    + inversion H_type; subst.
+      inversion H3; subst...
+  - inversion H_step; subst;
+    inversion H_type; subst...
+    all: inversion H7... 
+  - inversion H_step; subst;
+    inversion H_type; subst... 
+    Check test.
+    eapply test in H_type as [t_arg [H_t_v H_t_b]]...
+    (* TODO: 
+      Lemme sur le type des branches:
+      t_a -> t 
+      avec t_a le type associé au constructeur
+      
+    *)
+Qed.
