to_rewrite/okay/Subst.v
@@ -1,0 +1,341 @@
+From Coq Require Import Unicode.Utf8.
+From Coq Require Import Strings.String.
+Local Open Scope Z_scope.
+Require Import ZArith.
+Require Import Closed.
+Require Import Hints.
+
+Require Maps.
+Import Maps.Notations.
+Require Import Syntax.
+Require Import Types.
+Require Import List.
+Import ListNotations.
+
+
+Inductive substitution (s : expr) (x : string) : expr -> expr -> Prop :=
+  | S_Var_Eq :
+      substitution s x (E_Var x) s
+  | S_Var_Neq :
+      ∀ (y : string), x <> y -> substitution s x (E_Var y) (E_Var y)
+  | S_App : 
+      ∀ (e1 e1' e2 e2' : expr),
+      substitution s x e1 e1' ->
+      substitution s x e2 e2' ->
+      substitution s x (E_App e1 e2) (E_App e1' e2')
+  | S_Fun_Eq : 
+      ∀ (t : type) (e : expr),
+      substitution s x (E_Fun x t e) (E_Fun x t e)
+  | S_Fun_Neq : 
+      ∀ (y: string) (t : type) (e e' : expr),
+      x <> y ->
+      closed s ->
+      substitution s x e e' -> 
+      substitution s x (E_Fun y t e) (E_Fun y t e')
+  | S_True : 
+      substitution s x E_True E_True
+  | S_False : 
+      substitution s x E_False E_False
+  | S_If : 
+      ∀ (e1 e1' e2 e2' e3 e3' : expr),
+      substitution s x e1 e1' ->
+      substitution s x e2 e2' ->
+      substitution s x e3 e3' ->
+      substitution s x (E_If e1 e2 e3) (E_If e1' e2' e3')
+  | S_Let_Eq : 
+      ∀ (e1 e1' e2 : expr),
+      substitution s x e1 e1' -> 
+      substitution s x (E_Let x e1 e2) (E_Let x e1' e2)
+  | S_Let_Neq : 
+      ∀ (y : string) (e1 e1' e2 e2': expr),
+      x <> y ->
+      closed s ->
+      substitution s x e1 e1' -> 
+      substitution s x e2 e2' -> 
+      substitution s x (E_Let y e1 e2) (E_Let y e1' e2')
+  
+  | S_Num : 
+      ∀ (z : Z),
+      substitution s x (E_Num z) (E_Num z)
+  | S_Minus :
+      ∀ (e1 e1' e2 e2': expr),
+      substitution s x e1 e1' -> 
+      substitution s x e2 e2' -> 
+      substitution s x (E_Minus e1 e2) (E_Minus e1' e2')
+
+  | S_Eq :
+      ∀ (e1 e1' e2 e2': expr),
+      substitution s x e1 e1' -> 
+      substitution s x e2 e2' -> 
+      substitution s x (E_Eq e1 e2) (E_Eq e1' e2')
+  
+  | S_Pair : 
+      ∀ (e1 e1' e2 e2': expr),
+      substitution s x e1 e1' -> 
+      substitution s x e2 e2' -> 
+      substitution s x (E_Pair e1 e2) (E_Pair e1' e2')
+  | S_First :
+      ∀ (e e': expr),
+      substitution s x e e' -> 
+      substitution s x (E_First e) (E_First e')
+  | S_Second :
+      ∀ (e e': expr),
+      substitution s x e e' -> 
+      substitution s x (E_Second e) (E_Second e')
+
+  | S_Record_Nil : 
+      substitution s x E_Record_Nil E_Record_Nil
+    
+  | S_Record_Cons :
+    ∀ y e e' tail tail',
+    substitution s x tail tail' ->
+    substitution s x e e' ->
+    substitution s x (E_Record_Cons y e tail) (E_Record_Cons y e' tail')
+  
+  | S_Record_Access :
+    ∀ y e e',
+    substitution s x e e' ->
+    substitution s x (E_Record_Access e y) (E_Record_Access e' y)
+
+  | S_Fix :
+    ∀ e e',
+    substitution s x e e' -> 
+    substitution s x (E_Fix e) (E_Fix e')
+
+  | S_In_Left :
+      ∀ t₁ t₂ e e', 
+      substitution s x e e' ->
+      substitution s x (E_In_Left t₁ t₂ e) (E_In_Left t₁ t₂ e')
+  
+  | S_In_Right :
+      ∀ t₁ t₂ e e', 
+      substitution s x e e' ->
+      substitution s x (E_In_Right t₁ t₂ e) (E_In_Right t₁ t₂ e')
+
+  | S_Match :
+      ∀ e₁ e₂ e₃ e₁' e₂' e₃', 
+      substitution s x e₁ e₁' ->
+      substitution s x e₂ e₂' ->
+      substitution s x e₃ e₃' ->
+      substitution s x (E_Match e₁ e₂ e₃) (E_Match e₁' e₂' e₃')
+
+  | S_Unit : substitution s x E_Unit E_Unit
+  
+  | S_Sum_Constr :
+      ∀ constr e e',
+      substitution s x e e' ->
+      substitution s x (E_Sum_Constr constr e) (E_Sum_Constr constr e')
+
+  | S_Sum_Match :
+      ∀ e e' branches branches',
+      substitution s x e e' ->
+      substitution_lsexpr s x branches branches' -> 
+      substitution s x
+        (E_Sum_Match e branches) 
+        (E_Sum_Match e' branches')
+  
+  | S_Exc : 
+      ∀ exc, substitution s x (E_Exception exc) (E_Exception exc)
+
+with substitution_lsexpr (s : expr) (x : string) : lsexpr -> lsexpr -> Prop :=
+  | S_LSExpr_Nil : substitution_lsexpr s x LSE_Nil LSE_Nil
+  | S_LSExpr_Cons :
+    ∀ constr e e' branches branches', 
+    substitution s x e e' ->
+    substitution_lsexpr s x branches branches' ->
+    substitution_lsexpr s x 
+      (LSE_Cons constr e branches)
+      (LSE_Cons constr e' branches')
+.
+
+Hint Constructors substitution : local_hints.
+Hint Constructors substitution_lsexpr : local_hints.
+
+Check expr_ind.
+
+Fixpoint lookup_constr (constr : string) (branches : lsexpr) : option expr :=
+  match branches with
+  | LSE_Nil => None
+  | LSE_Cons constr' e tail =>
+      if (constr =? constr')%string 
+      then Some e 
+      else lookup_constr constr tail
+  end.
+
+
+Local Lemma exists_one : 
+  ∀ e s x, closed s -> 
+  ∃ e', substitution s x e e'.
+Proof with eauto with local_hints.
+  intros.
+  pose (
+    P (e : expr) :=
+      ∃ e', substitution s x e e'
+  ).
+  pose (
+    P0 (branches : lsexpr) :=
+      ∃ branches', substitution_lsexpr s x branches branches'
+  ).
+  apply expr_mut_ind with (P := P) (P0 := P0); unfold P; unfold P0; intros;
+  try (
+    try destruct H0; 
+    try destruct H1; 
+    try destruct H2;
+    try destruct (String.eqb_spec x x0); subst; 
+    eauto with local_hints; 
+    fail
+  ).
+Qed.
+
+Hint Resolve exists_one : local_hints.
+Search (_ = _ -> S _ = S _).
+
+Local Theorem deterministic :
+  ∀ e s x e'₁ e'₂, 
+  substitution s x e e'₁ ->
+  substitution s x e e'₂ ->
+  e'₁ = e'₂.
+Proof.
+  intro e.
+  pose (
+    P (e: expr) :=
+      ∀ s x e'₁ e'₂, 
+        substitution s x e e'₁ ->
+        substitution s x e e'₂ ->
+        e'₁ = e'₂
+  ).
+  pose (
+    P0 (branches: lsexpr) :=
+      ∀ s x branches'₁ branches'₂, 
+        substitution_lsexpr s x branches branches'₁ ->
+        substitution_lsexpr s x branches branches'₂ ->
+        branches'₁ = branches'₂
+  ).
+
+  apply expr_mut_ind with (P := P) (P0 := P0); unfold P; unfold P0; clear P P0;
+  try (
+    intros * H_s_1 H_s_2; inversion H_s_1; inversion H_s_2; subst;
+    eauto with local_hints;
+    try contradiction;
+    f_equal;
+    eapply IH; eauto with local_hints;
+    fail
+  );
+  try (
+    intros * IH * H_s_1 H_s_2; inversion H_s_1; inversion H_s_2; subst;
+    eauto with local_hints;
+    try contradiction;
+    f_equal;
+    eapply IH; eauto with local_hints;
+    fail
+  );
+  try (
+    intros * IH1 * IH2 * H_s_1 H_s_2; 
+    inversion H_s_1; inversion H_s_2; subst; 
+    eauto with local_hints;
+    try contradiction;
+    f_equal;
+    try (eapply IH1; eauto with local_hints; fail);
+    try (eapply IH2; eauto with local_hints; fail);
+    fail
+  );
+  try (
+    intros * IH1 * IH2 * IH3 * H_s_1 H_s_2; 
+    inversion H_s_1; inversion H_s_2; subst;
+    eauto with local_hints;
+    try contradiction; 
+    f_equal;
+    try (eapply IH1; eauto with local_hints; fail);
+    try (eapply IH2; eauto with local_hints; fail);
+    try (eapply IH3; eauto with local_hints; fail);
+    fail
+  ).
+  intros * H_s_1 H_s_2.
+  inversion H_s_1. inversion H_s_2; subst. destruct exc. destruct exc0. reflexivity.
+Qed.
+
+
+Local Theorem preserves_typing : 
+  ∀ e Γ Σ s x e' t_e t_s, 
+  has_type Σ (x |-> t_s; Γ)  e  t_e -> 
+  has_type Σ empty  s  t_s -> 
+  substitution s x e e' -> 
+  has_type Σ Γ e' t_e. 
+Proof with eauto with local_hints.
+  intro e.
+  pose (
+    P (e: expr) :=
+      ∀ Γ Σ s x e' t_e t_s, 
+      has_type Σ (x |-> t_s; Γ)  e  t_e -> 
+      has_type Σ empty  s  t_s -> 
+      substitution s x e e' -> 
+      has_type Σ Γ e' t_e
+  ).
+  pose (
+    P0 (branches: lsexpr) :=
+      ∀ name_sum Γ Σ s x branches' t_branches t_s, 
+      has_type_lsexpr name_sum Σ (x |-> t_s; Γ) branches t_branches -> 
+      has_type Σ empty s t_s -> 
+      substitution_lsexpr s x branches branches' -> 
+      has_type_lsexpr name_sum Σ Γ branches' t_branches
+  ).
+
+  apply expr_mut_ind with (P := P) (P0 := P0); unfold P; unfold P0;
+  clear P P0;
+  try (
+    intros * H_type_e H_type_s H_subst;
+    inversion H_subst; inversion H_type_e; subst;
+    eauto with local_hints;
+    fail
+  );
+  try (
+    intros * IH * H_type_e H_type_s H_subst;
+    inversion H_subst; inversion H_type_e; subst;
+    eauto with local_hints;
+    fail
+  );
+  try (
+    intros * IH1 * IH2 * H_type_e H_type_s H_subst;
+    inversion H_subst; inversion H_type_e; subst;
+    eauto with local_hints;
+    fail
+  );
+  try (
+    intros * IH1 * IH2 * IH3 * H_type_e H_type_s H_subst;
+    inversion H_subst; inversion H_type_e; subst;
+    eauto with local_hints;
+    fail
+  ).
+  - intros * H_type_e H_type_s H_subst.
+    inversion H_subst;
+    inversion H_type_e; inversion H4; subst.
+    + rewrite String.eqb_refl in *. inversion H7; subst...
+    + apply T_Var. rewrite <- H5. symmetry; apply Maps.update_neq...
+  - intros * IH * H_type_e H_type_s H_subst.
+    inversion H_subst;
+    inversion H_type_e; subst.
+    + apply T_Fun.
+      apply Types.weakening_eq with (Γ₁ := (x |-> t; x |-> t_s; Γ))...
+      apply Maps.update_shadow.
+    + apply T_Fun.
+      assert (has_type Σ (x0 |-> t_s; x |-> t; Γ) e0 t2) 
+      by (
+        apply Types.weakening_eq with (x |-> t; x0 |-> t_s; Γ);
+        try apply Maps.update_permute; eauto with local_hints
+      )...
+  - intros * IH1 * IH2 * H_type_e H_type_s H_subst.
+    inversion H_subst;
+    inversion H_type_e; subst.
+    + eapply T_Let.
+      * eapply IH1...
+      * apply Types.weakening_eq with ((x |-> t1; x |-> t_s; Γ));
+        try apply Maps.update_shadow...
+    + eapply T_Let.
+      * eapply IH1...
+      * assert (has_type Σ (x0 |-> t_s; x |-> t1; Γ) e2 t_e)
+        by (
+          apply Types.weakening_eq with (x |-> t1; x0 |-> t_s; Γ);
+          try apply Maps.update_permute; eauto with local_hints
+        )...  
+Qed.
+Hint Resolve preserves_typing : local_hints.
